Question 3 seems to be done

Labb2/Tokeneer/tokeneer.dfy
@@ -3,13 +3,82 @@ class Token{
   var cl : int;
 
   //for clearance: 0 = Low, 1 = Medium and 2 = High
+  //should -1 = invalid
   method Init(fingerPrint : int, clearance : int)
   modifies this;
-  requires 0 <= clearance <= 2;
+  requires validClearance(clearance);
   ensures fp == fingerPrint && cl == clearance;
   {
     fp := fingerPrint;
     cl := clearance;
   }
+  method InvalidateToken()
+  modifies this`cl;
+  ensures cl == -1;
+  {
+    cl := -1;
+  }
+  //Method to change clearance level?
+}
 
+class EnrollmentStn {
+  var fpSet : set<int>;
+
+  method Init()
+  modifies this;
+  //ensures fresh(fpSet);
+  {
+    fpSet := {};
+  }
+
+  method issueToken(fingerPrint : int, clearance : int) returns (t : Token)
+  modifies this`fpSet;
+  requires validClearance(clearance) && fingerPrint !in fpSet;
+  ensures fingerPrint in fpSet;
+  {
+    t := new Token;
+    t.Init(fingerPrint, clearance);
+    fpSet := fpSet + {fingerPrint};
+    return t;
+  }
+}
+class IDStn {
+  var clearanceLevel : int;
+  var alarm : bool;
+  var doorOpen : bool;
+
+  method Init(clearance : int)
+  modifies this;
+  requires validClearance(clearance);
+  ensures clearanceLevel == clearance && alarm == false && doorOpen == false;
+  {
+    clearanceLevel := clearance;
+    alarm := false;
+    doorOpen := false;
+  }
+
+  method tryOpenDoor(fingerPrint : int, t : Token)
+  modifies this`alarm, this`doorOpen, t;
+  requires t != null;
+  ensures alarm == true || doorOpen == true; //implement xor?
+  {
+    if(t.fp != fingerPrint || t.cl < clearanceLevel){
+      t.InvalidateToken();
+      alarm := true;
+    } else {
+      doorOpen := true;
+    }
+  }
+
+  method closeDoor()
+  modifies this`doorOpen;
+  ensures doorOpen == false;
+  {
+    doorOpen := false;
+  }
+}
+
+predicate validClearance(clearance : int)
+{
+   0 <= clearance <= 2
 }
